Architecture-independent characters, operator semantics, and bug fixes.
- Distinct character types, `char`, `wchar_t`, `char8_t`, `char16_t`, `char32_t`
  These have an architecture-independent representation using `Vchar`
- Integral promotion and fixes to the semantics of binary operators
- Fix an unsoundness where you could prove `False` in a program with a string literal containing `\0`

Contributions from @frantisek-bedrocksystems, @p-giarrusso, and @jhaag1.

include/Formatter.hpp
@@ -5,6 +5,7 @@
  */
 #pragma once
 
+#include "llvm/ADT/APSInt.h"
 #include "llvm/ADT/StringRef.h"
 #include "llvm/Support/raw_ostream.h"
 #include <string.h>
@@ -54,6 +55,8 @@ public:
 
 struct NBSP;
 extern const NBSP* nbsp;
+
+Formatter& operator<<(Formatter& out, const llvm::APSInt&);
 
 Formatter& operator<<(Formatter& out, const NBSP* _);
 
