theories/lang/cpp/logic/zstring.v
@@ -8,14 +8,10 @@ From Coq Require Import ZArith.BinInt Lists.List.
 
 From iris.proofmode Require Import proofmode.
 
-Require Import bedrock.prelude.stdpp_ssreflect.
-
 Require Import bedrock.prelude.base.
-From bedrock.lang.bi Require Import
-     prelude observe.
-From bedrock.lang.cpp Require Import
-     semantics.values
-     logic.arr logic.heap_pred logic.pred.
+From bedrock.lang.bi Require Import prelude observe.
+From bedrock.lang.cpp.semantics Require Import values.
+From bedrock.lang.cpp.logic Require Import arr heap_pred (* pred *).
 
 Import ChargeNotation.
 #[local] Open Scope Z_scope.
@@ -26,8 +22,12 @@ Import ChargeNotation.
     in C++. These arrays include the null-terminator
  *)
 Module zstring.
-  Definition t := list Z.
+  Definition t := list N.
   Bind Scope list_scope with t.
+
+Section with_ct.
+  Variable ct : char_type.
+  #[local] Notation Tchar := (Tchar_ ct).
 
   (* [size] reflects the in-memory footprint of the null-terminated string (i.e. the
      length is one greater than that of the string as given by `std::strlen`).
@@ -45,21 +45,47 @@ Module zstring.
   #[global] Arguments _strlen zs : simpl never.
   Notation strlen zs := (_strlen zs%Z).
 
+  Definition _WF_alt {σ : genv} (zs : t) : Prop :=
+    let zs' := take (length zs - 1) zs in
+    last zs = Some 0%N /\ 0%N ∉ zs' /\
+    List.Forall (λ c, 0 <= c < 2 ^ char_type.bitsN ct)%N zs'.
+  #[global] Instance _WF_alt_dec {σ : genv} zs : Decision (_WF_alt zs) := _.
+
   Definition _WF {σ : genv} (zs : t) : Prop :=
-    exists zs', zs = zs' ++ [0] /\ not (In 0 zs') /\
-    List.Forall (λ c : Z, has_type c Tuchar) zs.
+    exists zs', zs = zs' ++ [0]%N /\ not (In 0%N zs') /\
+    List.Forall (λ c : N, has_type (Vchar c) Tchar) zs.
   #[global] Arguments _WF {σ} zs : simpl never.
-  Notation WF zs := (_WF zs%Z).
+
+  Lemma _WF_WF_alt {σ : genv} zs : _WF zs <-> _WF_alt zs.
+  Proof.
+    rewrite /_WF /_WF_alt elem_of_list_In; setoid_rewrite <-has_type_char'; split. {
+      move=> [] zs' [] -> [].
+      rewrite last_app /= app_length Nat.add_sub take_app Forall_app Forall_singleton.
+      naive_solver.
+    }
+    move=> [] Hl [] Hin Hall; exists (take (length zs - 1) zs).
+    destruct zs as [|z zs] using rev_ind => //= {IHzs}.
+    move: Hl Hin Hall;
+      rewrite last_app app_length /=. rewrite Nat.add_sub take_app.
+      rewrite Forall_app Forall_singleton.
+    intros [= ->]; intros; split_and! => //.
+    lia.
+  Qed.
+
+  Notation WF zs := (_WF zs%N).
+  #[global, program] Instance _WF_dec {σ : genv} zs : Decision (_WF zs) :=
+    cast_if (decide (_WF_alt zs)).
+  Solve All Obligations with intros; exact /_WF_WF_alt.
 
   (* this definition is less intensional, and seems to work more
      smoothly wrt. automation: *)
   Definition _WF' {σ : genv} (zs : t) : Prop :=
     (exists v, nth_error zs 0 = Some v) /\
     (forall i, Z.of_nat i <= strlen zs ->
-          exists z, nth_error zs i = Some z /\ has_type (Vint z) Tuchar) /\
+          exists z, nth_error zs i = Some z /\ has_type (Vchar z) Tchar) /\
     (forall i, Z.of_nat i < strlen zs ->
-          exists z, nth_error zs i = Some z /\ z <> 0) /\
-    forall i, Z.of_nat i = strlen zs -> nth_error zs i = Some 0.
+          exists z, nth_error zs i = Some z /\ z <> 0%N) /\
+    forall i, Z.of_nat i = strlen zs -> nth_error zs i = Some 0%N.
   #[global] Arguments _WF' {σ} zs : simpl never.
   Notation WF' zs := (_WF' zs%Z).
 
@@ -72,17 +98,17 @@ Module zstring.
         eapply app_cons_not_nil; eauto.
     Qed.
 
-    Remark WF_singleton : WF [0].
+    Remark WF_singleton : WF [0%N].
     Proof.
       rewrite /_WF; exists []; repeat split.
       - intro CONTRA; by inversion CONTRA.
-      - repeat constructor; apply has_int_type; rewrite /bound/=; by lia.
+      - repeat constructor. apply has_type_char_0.
     Qed.
 
     Lemma WF_singleton_inj :
-      forall (z : Z),
+      forall (z : N),
         WF [z] ->
-        z = 0.
+        z = 0%N.
     Proof.
       intros * [zs [Hzs [Hin Hbounds]]].
       destruct zs; simpl in *; inversion Hzs.
@@ -102,9 +128,9 @@ Module zstring.
     Qed.
 
     Lemma WF_cons :
-      forall (z : Z) (zs : t),
-        (z <> 0)%Z ->
-        has_type (Vint z) Tuchar ->
+      forall (z : N) (zs : t),
+        (z <> 0)%N ->
+        has_type (Vchar z) Tchar ->
         WF (z :: zs) <->
         WF zs.
     Proof.
@@ -124,10 +150,27 @@ Module zstring.
           * by constructor.
     Qed.
 
+    (* Unlike WF_cons, here the explicit tail [++ [0]] lets us write a more elegant lemma. *)
+    Lemma WF_cons' (z : N) (zs : t) :
+      WF (z :: zs ++ [0%N]) <->
+      (z <> 0)%N /\ has_type (Vchar z) Tchar /\ WF (zs ++ [0%N]).
+    Proof.
+      rewrite /_WF/=. setoid_rewrite Forall_cons.
+      split.
+      - case => [[|z' zs'] [/= [-> Hzs']]]; first by destruct zs.
+        move: Hzs' => /(app_inj_2 _ _ _ _ eq_refl) [-> _].
+        move=> [/Decidable.not_or [Hz Hin] [Hz'Bounds Hrest]].
+        split_and! => //.
+        by exists zs'.
+      - case => Hz [HzBounds] [] zs' [] /(app_inj_2 _ _ _ _ eq_refl) [-> _] [Hin].
+        exists (z :: zs'); split_and! => //.
+        intros ?%in_inv. naive_solver.
+    Qed.
+
     (* WF is prefix-free predicate *)
     Lemma WF_eq_prefix_eq a1 a2 :
-      zstring.WF a1
-      -> zstring.WF a2
+      WF a1
+      -> WF a2
       -> a1 = take (length a1) a2
       -> a1 = a2.
     Proof.
@@ -165,13 +208,13 @@ Module zstring.
     Proof. by rewrite size_unfold. Qed.
 
     Lemma size_cons :
-      forall (z : Z) (zs : t),
+      forall (z : N) (zs : t),
         size (z :: zs) = 1 + size zs.
     Proof. intros *; rewrite !size_unfold/=; by lia. Qed.
 
     Lemma size_cons':
-      forall (z : Z) (zs : t),
-        (z <> 0)%Z ->
+      forall (z : N) (zs : t),
+        (z <> 0)%N ->
         WF (z :: zs) ->
         Z.to_nat (size (z :: zs)) = S (Z.to_nat (size zs)).
     Proof.
@@ -185,7 +228,6 @@ Module zstring.
     Qed.
 
     Lemma size_app :
-
       forall (zs zs' : t),
         size (zs ++ zs') = size zs + size zs'.
     Proof.
@@ -195,7 +237,7 @@ Module zstring.
     Qed.
 
     Lemma size_nil_cons_contra :
-      forall (z : Z) (zs : t),
+      forall (z : _) (zs : t),
         not (size (z :: zs) = size []).
     Proof. intros *; intro CONTRA; unfold size in CONTRA; by inversion CONTRA. Qed.
 
@@ -225,13 +267,13 @@ Module zstring.
     Proof. by rewrite strlen_unfold. Qed.
 
     Lemma strlen_cons (zs : t) :
-      forall (z : Z),
+      forall (z : _),
         strlen (z :: zs) = 1 + strlen zs.
     Proof. intros *; rewrite !strlen_unfold/=; by lia. Qed.
 
     Lemma strlen_cons':
-      forall (z : Z) (zs : t),
-        (z <> 0)%Z ->
+      forall (z : N) (zs : t),
+        (z <> 0)%N ->
         WF (z :: zs) ->
         Z.to_nat (strlen (z :: zs)) = S (Z.to_nat (strlen zs)).
     Proof.
@@ -255,7 +297,7 @@ Module zstring.
     Qed.
 
     Lemma strlen_nil_cons_contra :
-      forall (z : Z) (zs : t),
+      forall (z : _) (zs : t),
         not (strlen (z :: zs) = strlen []).
     Proof.
       intros *.
@@ -297,8 +339,8 @@ Module zstring.
     Section helpers.
       Lemma len0_take (zs : t)
             (H0 : 0 < List.length zs)
-            (H : forall i : nat, Z.of_nat i = strlen zs -> nth_error zs i = Some 0%Z) :
-        zs = take (List.length zs - 1) zs ++ [0%Z].
+            (H : forall i : nat, Z.of_nat i = strlen zs -> nth_error zs i = Some 0%N) :
+        zs = take (List.length zs - 1) zs ++ [0%N].
       Proof.
         rewrite -[zs](firstn_skipn (List.length zs - 1)). f_equal.
         { rewrite app_length take_length drop_length.
@@ -311,16 +353,16 @@ Module zstring.
         destruct zs; first by move: (H 1%nat eq_refl); inversion 1.
         apply: IH; first by simpl; lia.
         case; unfold strlen, size; rewrite /List.length -/List.length; first by lia.
-        move => n ?. simpl. move: (H (S (S n))). apply.
+        move => n' ?. simpl. move: (H (S (S n'))). apply.
         rewrite Nat2Z.inj_succ; unfold strlen, size; rewrite /List.length -/List.length. lia.
       Qed.
 
       Lemma forall_not0 (zs : t)
             (H : ∀ i : nat, (i <= strlen zs)%Z →
-                          ∃ z : Z, nth_error zs i = Some z ∧ has_type (Vint z) Tuchar)
+                          ∃ z : N, nth_error zs i = Some z ∧ has_type (Vchar z) Tchar)
             (H' : forall i : nat, (i < strlen zs)%Z ->
-                          ∃ z : Z, nth_error zs i = Some z /\ z <> 0):
-        List.Forall (fun z : Z => z <> 0 /\ has_type (Vint z) Tuchar) (take (List.length zs - 1) zs).
+                          ∃ z : N, nth_error zs i = Some z /\ z <> 0%N):
+        List.Forall (fun z : N => z <> 0%N /\ has_type (Vchar z) Tchar) (take (List.length zs - 1) zs).
       Proof.
         induction zs; first by constructor.
         simpl. have ->: (List.length zs - 0 = List.length zs)%nat by lia. destruct zs.
@@ -335,7 +377,7 @@ Module zstring.
               simpl in *; inversion H1; congruence. }
         have <-: (List.length zs - 0 = List.length zs)%nat by lia. apply: IHzs.
         case.
-        { move => h1; exists z. split => //.
+        { move => h1; exists n. split => //.
           destruct zs. 1: {
             specialize (H 1%nat ltac:(rewrite strlen_unfold/=; lia))
               as [z' [Hnth Htype]].
@@ -344,8 +386,8 @@ Module zstring.
           move: (H 1%nat); unfold strlen, size; case => //.
           { rewrite /List.length -/List.length. lia. }
             by move => x /=; case; inversion 1; subst. }
-        move => n; unfold strlen, size; rewrite /List.length -/List.length => h.
-        move: (H (S (S n))); case.
+        move => n'; unfold strlen, size; rewrite /List.length -/List.length => h.
+        move: (H (S (S n'))); case.
         { unfold strlen, size; rewrite /List.length -/List.length. lia. }
         move => x /=; case => h1 h2; exists x; split => //.
         intros i Hstrlen.
@@ -388,25 +430,25 @@ Module zstring.
           - specialize (h2 n ltac:(lia)) as [? ?]; intuition; congruence.
           - specialize (h4 n Hn).
             rewrite h4 in Hnth; inversion Hnth.
-            apply has_char_type; rewrite /bound/=; by lia.
+            apply has_type_char_0.
           - exfalso; eapply nth_error_strlen_contra; by eauto.
         }
-        suff: List.Forall (fun x => x <> 0 /\ has_type (σ:=σ) (Vint x) Tuchar)
+        suff: List.Forall (fun x => x <> 0%N /\ has_type (σ:=σ) (Vchar x) Tchar)
                           (take (Datatypes.length zs - 1) zs).
         { clear - zs. elim: zs => //= [_ [] //|a zs IH /=]. rewrite Nat.sub_0_r.
           destruct zs as [|z zs]; first done. move => /= /Forall_cons [[??]?].
           move => [//|]. simpl in IH. rewrite Nat.sub_0_r in IH. apply IH. done. }
         apply: forall_not0. apply h2. apply h3. }
       case => zs' []-> h1. split.
-      { destruct zs'; simpl; first by exists 0.
-                                          by exists z. }
+      { destruct zs'; simpl; first by exists 0%N.
+        by exists n. }
       split.
       { move => i. unfold strlen, size; rewrite app_length Nat2Z.inj_add /= => h2.
         assert (i < List.length zs' \/ i = List.length zs')%nat
           as [h2' | h2'] by lia; clear h2. 2: {
-          subst; exists 0; clear h1; split.
+          subst; exists 0%N; clear h1; split.
           - by induction zs'=> //=.
-          - by apply has_char_type; rewrite /bound/=; lia.
+          - apply has_type_char_0.
         }
         rewrite nth_error_app1 => //.
         elim: zs' i h1 h2' => /=; first by lia.
@@ -426,9 +468,9 @@ Module zstring.
         move => i; unfold strlen, size.
         rewrite app_length/=; intros Hi.
         assert (i < length zs')%nat as Hzs' by lia; clear Hi.
-        pose proof (nth_error_app1 zs' [0] Hzs') as Hnth.
-        pose proof (nth_In zs' 0 Hzs') as Hin.
-        rewrite Hnth; erewrite nth_error_nth' with (d:=0); eauto; eexists;
+        pose proof (nth_error_app1 zs' [0%N] Hzs') as Hnth.
+        pose proof (nth_In zs' 0%N Hzs') as Hin.
+        rewrite Hnth; erewrite nth_error_nth' with (d:=0%N); eauto; eexists;
           split; eauto.
         intro CONTRA; rewrite CONTRA in Hin.
         inversion h1; by congruence.
@@ -441,9 +483,9 @@ Module zstring.
     Qed.
 
     Lemma WF'_singleton_inj :
-      forall (z : Z),
+      forall (z : N),
         WF' [z] ->
-        z = 0.
+        z = 0%N.
     Proof. intros *; rewrite WFs_equiv; by apply WF_singleton_inj. Qed.
 
     Remark not_WF'_nil : not (WF' []).
@@ -456,9 +498,9 @@ Module zstring.
     Proof. intros *; rewrite WFs_equiv; by apply WF_nonempty_inj. Qed.
 
     Lemma WF'_cons :
-      forall (z : Z) (zs : t),
-        (z <> 0)%Z ->
-        has_type (Vint z) Tuchar ->
+      forall (z : _) (zs : t),
+        (z <> 0)%N ->
+        has_type (Vchar z) Tchar ->
         WF' (z :: zs) <->
         WF' zs.
     Proof. intros *; rewrite !WFs_equiv; by apply WF_cons. Qed.
@@ -471,15 +513,15 @@ Module zstring.
 
     Definition bufR (q : cQp.t) (sz : Z) (zs : t) : Rep :=
       [| size zs <= sz |] **
-      arrayR Tuchar (fun c => primR Tuchar q (Vint c)) zs ** [| WF zs |] **
-      .[Tuchar ! size zs]
-         |-> arrayR Tuchar (fun _ => primR Tuchar q 0) (repeat () (Z.to_nat (sz - size zs))).
+      arrayR Tchar (fun c => primR Tchar q (Vchar c)) zs ** [| WF zs |] **
+      .[Tchar ! size zs]
+         |-> arrayR Tchar (fun _ => primR Tchar q (Vchar 0)) (repeat () (Z.to_nat (sz - size zs))).
     (* The toplevel definition of [zstring.bufR']: *)
     Definition bufR' (q : cQp.t) (sz : Z) (zs : t) : Rep :=
       [| size zs <= sz |] **
-      arrayR Tuchar (fun c => primR Tuchar q (Vint c)) zs ** [| WF' zs |] **
-      .[Tuchar ! size zs]
-         |-> arrayR Tuchar (fun _ => primR Tuchar q 0) (repeat () (Z.to_nat (sz - size zs))).
+      arrayR Tchar (fun c => primR Tchar q (Vchar c)) zs ** [| WF' zs |] **
+      .[Tchar ! size zs]
+         |-> arrayR Tchar (fun _ => primR Tchar q (Vchar 0)) (repeat () (Z.to_nat (sz - size zs))).
 
     #[global] Instance bufR_WF_observe :
       forall q (sz : Z) (zs : t),
@@ -497,10 +539,10 @@ Module zstring.
 
     (* The toplevel definition of [zstring.R]: *)
     Definition R (q : cQp.t) (zs : t) : Rep :=
-      arrayR Tuchar (fun c => primR Tuchar q (Vint c)) zs ** [| WF zs |].
+      arrayR Tchar (fun c => primR Tchar q (Vchar c)) zs ** [| WF zs |].
     (* The toplevel definition of [zstring.R']: *)
     Definition R' (q : cQp.t) (zs : t) : Rep :=
-      arrayR Tuchar (fun c => primR Tuchar q (Vint c)) zs ** [| WF' zs |].
+      arrayR Tchar (fun c => primR Tchar q (Vchar c)) zs ** [| WF' zs |].
 
     #[global] Instance R_WF_observe :
       forall q (zs : t),
@@ -536,42 +578,42 @@ Module zstring.
         Proof. intros *; rewrite /Observe2/bufR; iIntros "%H [%CONTRA ?]"; by lia. Qed.
 
         #[global] Instance bufR_singleton :
-          forall (q : cQp.t) (sz : Z) (z : Z),
-            Observe [| z = 0 |]%Z (bufR q sz [z]).
+          forall (q : cQp.t) (sz : Z) (z : _),
+            Observe [| z = 0%N |] (bufR q sz [z]).
         Proof.
           intros *; rewrite /Observe/bufR; iIntros "(% & Hz & %HWF & rest)".
           iModIntro; iPureIntro; by apply WF_singleton_inj.
         Qed.
 
         Lemma bufR_cons :
-          forall (q : cQp.t) (sz : Z) (z : Z) (zs : t),
-            z <> 0 ->
+          forall (q : cQp.t) (sz : Z) (z : _) (zs : t),
+            z <> 0%N ->
             bufR q sz (z :: zs) -|-
-            primR Tuchar q z ** .[Tu8 ! 1] |-> bufR q (sz - 1) zs.
+            primR Tchar q (Vchar z) ** .[Tchar ! 1] |-> bufR q (sz - 1) zs.
         Proof.
           intros * Hz; split'.
           - rewrite /bufR arrayR_cons.
             iIntros "[%Hsz [[? [Hz Hzs]] [%HWF Hrest]]]".
             assert (size zs <= sz - 1) by (rewrite size_cons in Hsz; by lia).
-            iDestruct (observe [| has_type (Vint z) _ |] with "Hz") as "%".
+            iDestruct (observe [| has_type (Vchar z) _ |] with "Hz") as "%".
             assert (WF zs) by (apply WF_cons in HWF; assumption).
             rewrite !_offsetR_sep !_offsetR_only_provable
                     size_cons -_offsetR_sub_sub
-                    Z.sub_add_distr;
-              by iFrame "∗%".
+                    Z.sub_add_distr.
+              iFrame "∗%".
           - rewrite /bufR arrayR_cons !_offsetR_sep !_offsetR_only_provable;
               iIntros "[H [%Hsz [? [%HWF Hrest]]]]".
-            iDestruct (observe (type_ptrR Tuchar) with "H") as "#?".
+            iDestruct (observe (type_ptrR Tchar) with "H") as "#?".
             assert (size (z :: zs) <= sz) by (rewrite size_cons; by lia).
-            iDestruct (observe [| has_type (Vint z) _ |] with "H") as "%".
+            iDestruct (observe [| has_type (Vchar z) _ |] with "H") as "%".
             assert (WF (z :: zs)) by (apply WF_cons; assumption).
             rewrite size_cons -!_offsetR_sub_sub Z.sub_add_distr.
             iFrame "∗#%"; iPureIntro; by lia.
         Qed.
 
         #[global] Instance bufR_cons_cons_head_nonzero :
-          forall (q : cQp.t) (sz : Z) (z z' : Z) (zs : t),
-            Observe [| z <> 0 |]%Z (bufR q sz (z :: z' :: zs)).
+          forall (q : cQp.t) (sz : Z) (z z' : _) (zs : t),
+            Observe [| z <> 0 |]%N (bufR q sz (z :: z' :: zs)).
         Proof.
           intros *.
           apply: observe_intro_only_provable.
@@ -587,22 +629,22 @@ Module zstring.
           forall (q : cQp.t) (sz : Z) (zs : t),
             strlen zs < sz ->
                 bufR q sz zs
-            |-- bufR q sz zs ** [| List.Forall (fun c => has_type (Vint c) Tuchar) zs |].
+            |-- bufR q sz zs ** [| List.Forall (fun c => has_type (Vchar c) Tchar) zs |].
         Proof.
           intros **; generalize dependent sz; induction zs; intros **.
           - rewrite {1}bufR_nil; by iIntros.
           - destruct zs=> //=.
-            + iIntros "H"; iDestruct (observe [| a = 0 |]%Z with "H") as "%H'".
+            + iIntros "H"; iDestruct (observe [| a = 0 |]%N with "H") as "%H'".
               iFrame "∗"; iPureIntro.
               try repeat constructor; subst.
-              apply has_char_type; rewrite /bound; simpl in *; lia.
-            + iIntros "H"; iDestruct (observe [| WF (a :: z :: zs) |] with "H") as "%H'".
-              assert (1 <= size (a :: z :: zs)). {
+              apply has_type_char_0.
+            + iIntros "H"; iDestruct (observe [| WF (a :: n :: zs) |] with "H") as "%H'".
+              assert (1 <= size (a :: n :: zs)). {
                 rewrite -> size_cons in *.
-                pose proof (size_nonneg (z :: zs)).
+                pose proof (size_nonneg (n :: zs)).
                 by lia.
               }
-              iDestruct (observe [| a <> 0 |]%Z with "H") as "%H''"; iStopProof.
+              iDestruct (observe [| a <> 0 |]%N with "H") as "%H''"; iStopProof.
               rewrite {1}bufR_cons; auto; rewrite primR_has_type IHzs.
               iIntros "[[? %has_type] ?]"; iStopProof.
               rewrite _offsetR_sep _offsetR_only_provable.
@@ -610,14 +652,14 @@ Module zstring.
               rewrite -bufR_cons; [| done]; iFrame "∗"; iPureIntro.
               apply Forall_cons_2; auto.
               rewrite -> !strlen_cons in *.
-              pose proof (size_nonneg (z :: zs)).
+              pose proof (size_nonneg (n :: zs)).
               by lia.
         Qed.
 
         (* TODO (AUTO): Fix this once we add the correct observations for arrayR *)
         #[global] Instance bufR_type_ptrR_observe :
           forall q (sz : Z) (zs : t),
-            Observe (type_ptrR Tu8) (bufR q sz zs).
+            Observe (type_ptrR Tchar) (bufR q sz zs).
         Proof.
           move=> q sz zs; rewrite /bufR; destruct zs.
           - rewrite /Observe. iIntros "[? [? [%CONTRA ?]]]";
@@ -627,24 +669,24 @@ Module zstring.
 
         #[global] Instance bufR_validR_end_observe :
           forall q (sz : Z) (zs : t),
-            Observe (.[Tuchar ! sz] |-> validR) (bufR q sz zs).
+            Observe (.[Tchar ! sz] |-> validR) (bufR q sz zs).
         Proof.
           move=> q sz zs; rewrite /bufR/Observe.
           iIntros "[%Hsz [array [%HWF rest]]]".
-          iAssert (arrayR Tuchar (fun c => primR Tuchar q (Vint c))
-                          (zs ++ repeat 0 (Z.to_nat (sz - size zs))))
+          iAssert (arrayR Tchar (fun c => primR Tchar q (Vchar c))
+                          (zs ++ repeat 0%N (Z.to_nat (sz - size zs))))
             with "[array rest]" as "array'". 2: {
-            assert (Z.to_nat sz <= length (zs ++ repeat 0%Z (Z.to_nat (sz - size zs))))%nat
+            assert (Z.to_nat sz <= length (zs ++ repeat 0%N (Z.to_nat (sz - size zs))))%nat
               as AUX. 1: {
               rewrite app_length repeat_length.
               unfold strlen in Hsz.
               unfold size in *.
               lia.
             }
-            pose proof (arrayR_valid_obs (λ c : Z, primR Tuchar q c) Tuchar (Z.to_nat sz)
-                                         (zs ++ repeat 0 (Z.to_nat (sz - size zs)))
+            pose proof (arrayR_valid_obs (λ c : N, primR Tchar q (Vchar c)) Tchar (Z.to_nat sz)
+                                         (zs ++ repeat 0%N (Z.to_nat (sz - size zs)))
                                          AUX).
-            iDestruct (observe (.[ Tnum char_bits Unsigned ! sz ] |-> validR) with "array'")
+            iDestruct (observe (.[ Tchar ! sz ] |-> validR) with "array'")
               as "#?"; auto.
             rewrite Z2Nat.id in H; auto.
             pose proof (size_nonneg zs).
@@ -663,7 +705,7 @@ Module zstring.
         #[global] Instance bufR_validR_inbounds_observe :
           forall q sz (z : Z) (zs : t),
             (0 <= z <= sz)%Z ->
-            Observe (.[Tuchar ! z] |-> validR) (bufR q sz zs).
+            Observe (.[Tchar ! z] |-> validR) (bufR q sz zs).
         Proof.
           intros **; generalize dependent zs; induction z; intros **; simpl in *.
           - rewrite ->o_sub_0 by eauto; rewrite _offsetR_id; refine _.
@@ -675,14 +717,14 @@ Module zstring.
             assert (z <= length zs \/ length zs < z)%Z
               as [Hz' | Hz'] by lia.
             + iClear "zeros".
-              iDestruct (observe (.[Tnum char_bits Unsigned ! z] |-> validR) with "zs")
+              iDestruct (observe (.[ Tchar ! z] |-> validR) with "zs")
                 as "#valid"; last by iFrame "#".
               pose proof (arrayR_valid_obs
-                            (fun c => primR (Tnum char_bits Unsigned) q (Vint c))
-                            (Tnum char_bits Unsigned) (Z.to_nat z) zs ltac:(lia)).
+                            (fun c => primR Tchar q (Vchar c))
+                            Tchar (Z.to_nat z) zs ltac:(lia)).
               by rewrite ->Z2Nat.id in H0 by lia.
             + iClear "zs".
-              iDestruct (observe (.[Tnum char_bits Unsigned ! z] |-> validR) with "zeros")
+              iDestruct (observe (.[Tchar ! z] |-> validR) with "zeros")
                 as "#valid"; last by iFrame "#".
               assert (exists z', size zs + z' = z /\ 0 <= z')
                 as [z' [Hz'' Hneg]]
@@ -690,8 +732,8 @@ Module zstring.
                 subst.
               rewrite -_offsetR_sub_sub; apply _offsetR_observe.
               pose proof (arrayR_valid_obs
-                            (fun c => primR (Tnum char_bits Unsigned) q 0)
-                            (Tnum char_bits Unsigned) (Z.to_nat z')
+                            (fun c => primR Tchar q (Vchar 0))
+                            Tchar (Z.to_nat z')
                             (repeat () (Z.to_nat (sz - size zs)))
                             ltac:(rewrite repeat_length; lia)).
               by rewrite ->Z2Nat.id in H0 by lia.
@@ -713,44 +755,44 @@ Module zstring.
         Proof. lift_WF2WF' bufR_sz_contra. Qed.
 
         #[global] Instance bufR'_singleton :
-          forall (q : cQp.t) (sz : Z) (z : Z),
+          forall (q : cQp.t) (sz : Z) (z : _),
             0 <= sz ->
-            Observe [| z = 0 |]%Z (bufR' q sz [z]).
+            Observe [| z = 0 |]%N (bufR' q sz [z]).
         Proof. lift_WF2WF' bufR_singleton. Qed.
 
         Lemma bufR'_cons :
-          forall (q : cQp.t) (sz : Z) (z : Z) (zs : t),
-            z <> 0 ->
+          forall (q : cQp.t) (sz : Z) (z : _) (zs : t),
+            z <> 0%N ->
             bufR' q sz (z :: zs) -|-
-            primR Tuchar q z ** .[Tu8 ! 1] |-> bufR' q (sz - 1) zs.
+            primR Tchar q (Vchar z) ** .[Tchar ! 1] |-> bufR' q (sz - 1) zs.
         Proof. lift_WF2WF' bufR_cons. Qed.
 
         #[global] Instance bufR'_cons_cons_head_nonzero :
-          forall (q : cQp.t) (sz : Z) (z z' : Z) (zs : t),
-            Observe [| z <> 0 |]%Z (bufR' q sz (z :: z' :: zs)).
+          forall (q : cQp.t) (sz : Z) (z z' : _) (zs : t),
+            Observe [| z <> 0 |]%N (bufR' q sz (z :: z' :: zs)).
         Proof.  lift_WF2WF' bufR_cons_cons_head_nonzero. Qed.
 
         Lemma bufR'_has_type :
           forall (q : cQp.t) (sz : Z) (zs : t),
             strlen zs < sz ->
                 bufR' q sz zs
-            |-- bufR' q sz zs ** [| List.Forall (fun c => has_type (Vint c) Tuchar) zs |].
+            |-- bufR' q sz zs ** [| List.Forall (fun c => has_type (Vchar c) Tchar) zs |].
         Proof. lift_WF2WF' bufR_has_type. Qed.
 
         #[global] Instance bufR'_type_ptrR_observe :
           forall q (sz : Z) (zs : t),
-            Observe (type_ptrR Tu8) (bufR' q sz zs).
+            Observe (type_ptrR Tchar) (bufR' q sz zs).
         Proof. lift_WF2WF' bufR_type_ptrR_observe. Qed.
 
         #[global] Instance bufR'_validR_end_observe :
           forall q (sz : Z) (zs : t),
-            Observe (.[Tuchar ! sz] |-> validR) (bufR' q sz zs).
+            Observe (.[Tchar ! sz] |-> validR) (bufR' q sz zs).
         Proof. lift_WF2WF' bufR_validR_end_observe. Qed.
 
         #[global] Instance bufR'_validR_inbounds_observe :
           forall q sz (z : Z) (zs : t),
             (0 <= z <= sz)%Z ->
-            Observe (.[Tuchar ! z] |-> validR) (bufR' q sz zs).
+            Observe (.[Tchar ! z] |-> validR) (bufR' q sz zs).
         Proof. lift_WF2WF' bufR_validR_inbounds_observe. Qed.
       End bufR'.
 
@@ -758,7 +800,7 @@ Module zstring.
         forall (q : cQp.t) (sz : Z) (zs : t),
           bufR q sz zs -|-
           [| size zs <= sz |] ** R q zs **
-          .[ Tuchar ! size zs] |-> arrayR Tuchar (fun _ => primR Tuchar q 0)
+          .[ Tchar ! size zs] |-> arrayR Tchar (fun _ => primR Tchar q (Vchar 0))
                                            (repeat () (Z.to_nat (sz - size zs))).
       Proof.
         intros **; split'.
@@ -770,7 +812,7 @@ Module zstring.
         forall (q : cQp.t) (sz : Z) (cstr : t),
           bufR' q sz cstr -|-
           [| size cstr <= sz |] ** R' q cstr **
-          .[ Tuchar ! size cstr] |-> arrayR Tuchar (fun _ => primR Tuchar q 0)
+          .[ Tchar ! size cstr] |-> arrayR Tchar (fun _ => primR Tchar q (Vchar 0))
                                              (repeat () (Z.to_nat (sz - size cstr))).
       Proof. intros **; rewrite -!bufRs_equiv -!Rs_equiv; by apply bufR_unfold. Qed.
 
@@ -783,7 +825,7 @@ Module zstring.
           - iIntros "[array %HWF]".
             assert (size zs <= size zs) by lia.
             rewrite Z.sub_diag/= arrayR_nil.
-            iDestruct (observe (.[Tuchar ! size zs] |-> validR) with "array") as "#?". 1: {
+            iDestruct (observe (.[Tchar ! size zs] |-> validR) with "array") as "#?". 1: {
               unfold size; apply arrayR_valid_obs; by lia.
             }
             rewrite _offsetR_sep _offsetR_only_provable;
@@ -798,15 +840,15 @@ Module zstring.
         Proof. try_lift_bufR bufR_nil. Qed.
 
         #[global] Instance R_singleton :
-          forall (q : cQp.t) (z : Z),
-            Observe [| z = 0 |]%Z (R q [z]).
+          forall (q : cQp.t) (z : _),
+            Observe [| z = 0 |]%N (R q [z]).
         Proof. try_lift_bufR bufR_singleton. Qed.
 
         Lemma R_cons :
-          forall (q : cQp.t) (z : Z) (zs : t),
-            z <> 0 ->
+          forall (q : cQp.t) (z : _) (zs : t),
+            z <> 0%N ->
             R q (z :: zs) -|-
-            primR Tuchar q z ** .[Tu8 ! 1] |-> R q zs.
+            primR Tchar q (Vchar z) ** .[Tchar ! 1] |-> R q zs.
         Proof.
           intros **; rewrite !R_bufR_equiv.
           replace (size zs) with ((size (z :: zs)) - 1)
@@ -815,14 +857,14 @@ Module zstring.
         Qed.
 
         #[global] Instance R_cons_cons_head_nonzero :
-          forall (q : cQp.t) (z z' : Z) (zs : t),
-            Observe [| z <> 0 |]%Z (R q (z :: z' :: zs)).
+          forall (q : cQp.t) (z z' : _) (zs : t),
+            Observe [| z <> 0 |]%N (R q (z :: z' :: zs)).
         Proof. try_lift_bufR bufR_cons_cons_head_nonzero. Qed.
 
         Lemma R_has_type :
           forall (q : cQp.t) (zs : t),
                 R q zs
-            |-- R q zs ** [| List.Forall (fun c => has_type (Vint c) Tuchar) zs |].
+            |-- R q zs ** [| List.Forall (fun c => has_type (Vchar c) Tchar) zs |].
         Proof.
           try_lift_bufR bufR_has_type.
           unfold strlen; by lia.
@@ -831,17 +873,17 @@ Module zstring.
         (* TODO (AUTO): Fix this once we add the correct observations for arrayR *)
         #[global] Instance R_type_ptrR_observe :
           forall q (zs : t),
-            Observe (type_ptrR Tu8) (R q zs).
+            Observe (type_ptrR Tchar) (R q zs).
         Proof. try_lift_bufR bufR_type_ptrR_observe. Qed.
 
         #[global] Instance R_validR_end_observe :
           forall q (zs : t),
-            Observe (.[Tuchar ! size zs] |-> validR) (R q zs).
+            Observe (.[Tchar ! size zs] |-> validR) (R q zs).
         Proof. try_lift_bufR bufR_validR_end_observe. Qed.
 
         #[global] Instance R_validR_end_observe' :
           forall q (zs : t),
-            Observe (.[Tuchar ! strlen zs] |-> .[Tuchar ! 1] |-> validR) (R q zs).
+            Observe (.[Tchar ! strlen zs] |-> .[Tchar ! 1] |-> validR) (R q zs).
         Proof.
           intros *; pose proof (R_validR_end_observe q zs).
           rewrite _offsetR_sub_sub; unfold size, strlen in *.
@@ -854,13 +896,13 @@ Module zstring.
         #[global] Instance R_validR_inbounds_observe :
           forall q (z : Z) (zs : t),
             (0 <= z <= size zs)%Z ->
-            Observe (.[Tuchar ! z] |-> validR) (R q zs).
+            Observe (.[Tchar ! z] |-> validR) (R q zs).
         Proof.
           intros * Hsize; unfold R; unfold size in Hsize.
           apply observe_sep_l.
           pose proof (arrayR_valid_obs
-                        (fun c => primR (Tnum char_bits Unsigned) q (Vint c))
-                        (Tnum char_bits Unsigned) (Z.to_nat z) zs ltac:(lia)).
+                        (fun c => primR Tchar q (Vchar c))
+                        Tchar (Z.to_nat z) zs ltac:(lia)).
           by rewrite ->Z2Nat.id in H by lia.
         Qed.
       End R_Theory.
@@ -878,63 +920,71 @@ Module zstring.
         Proof. lift_WF2WF' R_nil. Qed.
 
         #[global] Instance R'_singleton :
-          forall (q : cQp.t) (z : Z),
-            Observe [| z = 0 |]%Z (R' q [z]).
+          forall (q : cQp.t) (z : _),
+            Observe [| z = 0 |]%N (R' q [z]).
         Proof. lift_WF2WF' R_singleton. Qed.
 
         Lemma R'_cons :
-          forall (q : cQp.t) (z : Z) (zs : t),
-            z <> 0 ->
+          forall (q : cQp.t) (z : _) (zs : t),
+            z <> 0%N ->
             R' q (z :: zs) -|-
-            primR Tuchar q z ** .[Tu8 ! 1] |-> R' q zs.
+            primR Tchar q (Vchar z) ** .[Tchar ! 1] |-> R' q zs.
         Proof. lift_WF2WF' R_cons. Qed.
 
         #[global] Instance R'_cons_cons_head_nonzero :
-          forall (q : cQp.t) (z z' : Z) (zs : t),
-            Observe [| z <> 0 |]%Z (R' q (z :: z' :: zs)).
+          forall (q : cQp.t) (z z' : _) (zs : t),
+            Observe [| z <> 0 |]%N (R' q (z :: z' :: zs)).
         Proof. lift_WF2WF' R_cons_cons_head_nonzero. Qed.
 
         Lemma R'_has_type :
           forall (q : cQp.t) (zs : t),
                 R' q zs
-            |-- R' q zs ** [| List.Forall (fun c => has_type (Vint c) Tuchar) zs |].
+            |-- R' q zs ** [| List.Forall (fun c => has_type (Vchar c) Tchar) zs |].
         Proof. lift_WF2WF' R_has_type. Qed.
 
         #[global] Instance R'_type_ptrR_observe :
           forall q (zs : t),
-            Observe (type_ptrR Tu8) (R' q zs).
+            Observe (type_ptrR Tchar) (R' q zs).
         Proof. lift_WF2WF' R_type_ptrR_observe. Qed.
 
         #[global] Instance R'_validR_end_observe :
           forall q (zs : t),
-            Observe (.[Tuchar ! size zs] |-> validR) (R' q zs).
+            Observe (.[Tchar ! size zs] |-> validR) (R' q zs).
         Proof. lift_WF2WF' R_validR_end_observe. Qed.
 
         #[global] Instance R'_validR_end_observe' :
           forall q (zs : t),
-            Observe (.[Tuchar ! strlen zs] |-> .[Tuchar ! 1] |-> validR) (R' q zs).
+            Observe (.[Tchar ! strlen zs] |-> .[Tchar ! 1] |-> validR) (R' q zs).
         Proof. lift_WF2WF' R_validR_end_observe'. Qed.
 
         #[global] Instance R'_validR_inbounds_observe :
           forall q (z : Z) (zs : t),
             (0 <= z <= size zs)%Z ->
-            Observe (.[Tuchar ! z] |-> validR) (R' q zs).
+            Observe (.[Tchar ! z] |-> validR) (R' q zs).
         Proof. lift_WF2WF' R_validR_inbounds_observe. Qed.
       End R'_Theory.
 
       Lemma R_unfold :
         forall (q : cQp.t) (zs : t),
               R q zs
-          -|- arrayR Tuchar (fun c => primR Tuchar q (Vint c)) zs ** [| WF zs |].
+          -|- arrayR Tchar (fun c => primR Tchar q (Vchar c)) zs ** [| WF zs |].
       Proof. intros **; split'; by rewrite /R. Qed.
 
       Lemma R'_unfold :
         forall (q : cQp.t) (zs : t),
               R' q zs
-          -|- arrayR Tuchar (fun c => primR Tuchar q (Vint c)) zs ** [| WF' zs |].
+          -|- arrayR Tchar (fun c => primR Tchar q (Vchar c)) zs ** [| WF' zs |].
       Proof. intros **; split'; by rewrite /R'. Qed.
     End Theory.
   End with_Σ.
+End with_ct.
+
+(* refresh notation outside of the section *)
+Notation size zs := (_size zs%Z).
+Notation strlen zs := (_strlen zs%Z).
+Notation WF zs := (_WF zs%Z).
+Notation WF' zs := (_WF' zs%Z).
+
 End zstring.
 
 Section zstring_pure_hint_test_pre.
@@ -953,7 +1003,7 @@ Section zstring_pure_hint_test_pre.
   Abort.
   #[local] Unset Ltac Backtrace.
 
-  Goal forall {σ : genv}, not (zstring.WF []).
+  Goal forall {σ : genv}, not (zstring.WF char_type.Cchar []).
   Proof. Fail (by auto with pure). Abort.
 
   Goal
@@ -987,7 +1037,7 @@ End zstring_pure_hint_test_pre.
 Section zstring_pure_hint_test_post.
   #[local] Unset Ltac Backtrace.
 
-  Goal forall {σ : genv}, not (zstring.WF []).
+  Goal forall {σ : genv}, not (zstring.WF char_type.Cchar []).
   Proof. by auto with pure. Abort.
 
   Goal
