theories/lang/cpp/logic/core_string.v
@@ -1,0 +1,54 @@
+(*
+ * Copyright (C) BedRock Systems Inc. 2023
+
+ * This software is distributed under the terms of the BedRock Open-Source License.
+ * See the LICENSE-BedRock file in the repository root for details.
+ *)
+Require Import elpi.apps.locker.
+From iris.proofmode Require Import proofmode.
+
+From bedrock.lang.bi Require Import prelude observe.
+From bedrock.lang.cpp.semantics Require Import values.
+From bedrock.lang.cpp.logic Require Import arr heap_pred.
+From bedrock.lang.cpp.bi Require Import spec.
+
+Import ChargeNotation.
+#[local] Open Scope Z_scope.
+
+(** Core C++ string theory: part of the semantics. *)
+
+(** [strings_bytesR ct q chars] is [q] (const) fractional ownership of
+    [chars] with a trailing [0].
+    - Unlike [zstring.t], does not assume the contents avoid `0` elements, since that property might not be guaranteed in all character types/encodings.
+    - Used for string literals of arbitrary character types.
+
+    NOTE that [chars] is in units of *characters* using the standard
+          character encoding (see [syntax/expr.v]). This is *not* the
+          same as bytes, and will not be for multi-byte characters.
+  *)
+mlock
+Definition string_bytesR `{Σ : cpp_logic} {σ : genv} (cty : char_type) (q : cQp.t) (ls : list N) : Rep :=
+  let ty := Tchar_ cty in
+  arrayR ty (λ c, primR ty q (N_to_char cty c)) (ls ++ [0%N]).
+#[global] Arguments string_bytesR {_ _ _} _ _ _ : assert.
+
+(* Arguments char_type.bitsN !_ /.
+Arguments char_type.bytesN !_ /. *)
+Lemma N_to_char_Cchar_eq (c : N) :
+  (c < 2 ^ 8)%N ->
+  N_to_char char_type.Cchar c = Vchar c.
+Proof.
+  intros.
+  rewrite /N_to_char /operator.trimN/=. f_equiv.
+  exact: N.mod_small.
+Qed.
+
+Section with_Σ.
+  Context `{Σ : cpp_logic} {σ : genv}.
+
+  #[global] Instance string_bytesR_timeless : Timeless3 string_bytesR.
+  Proof. rewrite string_bytesR.unlock /=. apply _. Qed.
+
+  #[global] Instance string_bytesR_cfrac cty : CFractional1 (string_bytesR cty).
+  Proof. rewrite string_bytesR.unlock /=. apply _. Qed.
+End with_Σ.
