theories/lang/cpp/logic/string.v
@@ -4,6 +4,7 @@
  * This software is distributed under the terms of the BedRock Open-Source License.
  * See the LICENSE-BedRock file in the repository root for details.
  *)
+Require Export bedrock.lang.cpp.logic.core_string.
 Require Export bedrock.lang.cpp.logic.cstring.
 Require Export bedrock.lang.cpp.logic.zstring.
 
