theories/lang/cpp/semantics.v
@@ -6,7 +6,10 @@
 From bedrock.lang.cpp.semantics Require Export
      sub_module
      values
+     cast
      operator
      intensional
+     promotion
+     cast_operator
      subtyping
      dispatch.
