theories/lang/cpp/semantics/cast.v
@@ -1,0 +1,223 @@
+(*
+ * Copyright (c) 2020-23 BedRock Systems, Inc.
+ * This software is distributed under the terms of the BedRock Open-Source License.
+ * See the LICENSE-BedRock file in the repository root for details.
+ *)
+(** ** Primitive Conversions
+
+    This file covers conversions between primitive types.
+ *)
+From elpi Require Import locker.
+
+From bedrock.prelude Require Import base numbers.
+From bedrock.lang.cpp.arith Require Export operator.
+From bedrock.lang.cpp Require Import ast.
+From bedrock.lang.cpp.semantics Require Import values genv promotion characters.
+Export characters.
+
+#[local] Open Scope Z_scope.
+
+(** Numeric conversions.
+
+    This includes both conversions and promotions between fundamental
+    numeric types and enumerations (which have underlying fundamental
+    types).
+
+    This relation only holds on well-typed values, see [conv_int_well_typed].
+  *)
+Definition conv_int {σ : genv} (tu : translation_unit) (from to : type) (v v' : val) : Prop :=
+  has_type v from /\
+  match representation_type tu from , representation_type tu to with
+  | Tbool , Tnum _ _ =>
+      match is_true v with
+      | Some v => v' = Vbool v
+      | _ => False
+      end
+  | Tbool , Tchar_ _ =>
+      match is_true v with
+      | Some v => v' = Vchar (if v then 1 else 0)%N
+      | _ => False
+      end
+  | Tnum _ _ , Tbool =>
+      match v with
+      | Vint v => v' = Vbool (bool_decide (v <> 0))
+      | _ => False
+      end
+  | Tnum _ _ , Tnum sz Unsigned =>
+      match v with
+      | Vint v => v' = Vint (to_unsigned sz v)
+      | _ => False
+      end
+  | Tnum _ _ , Tnum sz Signed =>
+      has_type v (Tnum sz Signed) /\ v' = v
+  | Tbool , Tbool => v = v'
+  | Tchar_ _ , Tbool =>
+      match v with
+      | Vchar v => v' = Vbool (bool_decide (v <> 0%N))
+      | _ => False
+      end
+  | Tnum sz sgn , Tchar_ ct =>
+      match v with
+      | Vint v =>
+          v' = Vchar (to_char (bitsN sz) sgn (char_type.bitsN ct) v)
+      | _ => False
+      end
+  | Tchar_ ct , Tnum sz sgn =>
+      match v with
+      | Vchar v => v' = Vint (of_char (char_type.bitsN ct) (signedness_of_char σ ct) (bitsN sz) sgn v)
+      | _ => False
+      end
+  | Tchar_ ct , Tchar_ ct' =>
+      match v with
+      | Vchar v => v' = Vchar (to_char (char_type.bitsN ct) Unsigned (char_type.bitsN ct') v)
+      | _ => False
+      end
+  | Tenum _ , _
+  | _ , Tenum _ (* not reachable due to [representation_type] *)
+  | _ , _ => False
+  end.
+Arguments conv_int !_ !_ _ _ /.
+
+Section conv_int.
+  Context `{Hmod : tu ⊧ σ}.
+
+  (* TODO move *)
+  Lemma has_type_representation_type ty v :
+    has_type v ty -> has_type v (representation_type tu ty).
+  Proof using Hmod.
+    induction ty; rewrite /representation_type /= //.
+    { intros.
+      rewrite /underlying_type.
+      case_match => //.
+      case_match => //.
+      eapply has_type_enum in H.
+      destruct H as [?[?[?[?[??]]]]].
+      subst.
+      generalize (enum_compat (ODR Hmod H _ _ _ H0 H2)); intro; subst.
+      tauto. }
+    { intros.
+      apply has_type_qual_iff in H.
+      by apply IHty. }
+  Qed.
+
+  Lemma has_type_representation_type_not_raw ty v :
+    ~is_raw v ->
+    has_type v ty <-> has_type v (representation_type tu ty).
+  Proof using Hmod.
+    induction ty; rewrite /representation_type /= //.
+    { split; intros.
+      { rewrite /underlying_type.
+        case_match => //.
+        case_match => //.
+        eapply has_type_enum in H0.
+        destruct H0 as [?[?[?[?[??]]]]].
+        subst.
+        generalize (enum_compat (ODR Hmod H0 _ _ _ H1 H3)); intro; subst.
+        tauto. }
+      { unfold underlying_type in H0.
+        case_match; simpl in *; eauto.
+        case_match; simpl in *; eauto.
+        apply has_type_enum. do 3 eexists; split; eauto. } }
+    { intros.
+      apply IHty in H.
+      rewrite -has_type_qual_iff. apply H. }
+  Qed.
+  (* END MOVE *)
+
+  Lemma conv_int_well_typed ty ty' v v' :
+       tu ⊧ σ -> (* TODO only needed if either type is a [Tenum] *)
+       conv_int tu ty ty' v v' ->
+       has_type v ty /\ has_type v' ty'.
+  Proof using Hmod.
+    rewrite /conv_int.
+    destruct (representation_type tu ty) eqn:src_ty; rewrite /=; try tauto;
+    destruct (representation_type tu ty') eqn:dst_ty; rewrite /=; try tauto;
+    intuition;
+    match goal with
+    | H : representation_type ?tu ?ty = ?ty' , H' : has_type _ ?ty |- _ =>
+        generalize (has_type_representation_type _ _ H'); rewrite H; intro
+    end; repeat (case_match; try tauto);
+      repeat match goal with
+        | H : _ /\ _ |- _ => destruct H
+        | H : exists x, _ |- _ => destruct H
+        | H : representation_type _ ?ty = ?ty2 |- has_type _ ?ty =>
+            eapply has_type_representation_type_not_raw => /=; try congruence; try rewrite H
+        end; subst; eauto.
+    { destruct v; simpl; try tauto.
+      eapply has_int_type' in H2.
+      destruct H2 as [[?[??]] | [?[??]]]; congruence. }
+    { eapply has_int_type.
+      red; rewrite /=/max_val/trim.
+      generalize (Z_mod_lt z (2 ^ bitsN size0) ltac:(lia)).
+      destruct size0 => /=; try lia. }
+    { eapply has_type_char.
+      eexists; split; eauto.
+      rewrite to_char.unlock.
+      generalize (Z_mod_lt z (2 ^ char_type.bitsN t) ltac:(lia)).
+      destruct t; try lia. }
+    { eapply has_bool_type. case_match; lia. }
+    { eapply has_int_type.
+      eapply has_type_char' in H0.
+      red.
+      generalize (of_char_bounded (char_type.bitsN t) (signedness_of_char σ t) (bitsN size) signed n
+                    ltac:(destruct size; simpl; lia)
+                    ltac:(destruct t; simpl; lia)).
+      rewrite /min_val/max_val. repeat case_match; simpl; lia. }
+    { apply has_type_char; eexists; split; eauto.
+      apply has_type_char in H0.
+      destruct H0 as [?[Hinv?]]; inversion Hinv; subst.
+      generalize (to_char_bounded (char_type.bitsN t) Unsigned (char_type.bitsN t0) (Z.of_N x)); eauto. }
+    { eapply has_bool_type; case_match; lia. }
+    { eapply has_int_type. red; destruct size, signed, b => /=; lia. }
+    { eapply has_type_char'. destruct t => /=; lia. }
+    { eapply has_type_char; eexists; split; eauto. destruct t => /=; lia. }
+    { eapply has_type_bool in H0.
+      destruct H0. subst. simpl. tauto. }
+  Qed.
+
+  (* Note that a no-op conversion on a raw value is not permitted. *)
+  Lemma conv_int_num_id sz sgn v :
+    let ty := Tnum sz sgn in
+    ~(exists r, v = Vraw r) ->
+    has_type v ty ->
+    conv_int tu ty ty v v.
+  Proof using Hmod.
+    rewrite /=/conv_int/underlying_type/=.
+    intros. split; eauto.
+    destruct sgn. split; eauto.
+    apply has_int_type' in H0.
+    destruct H0.
+    - destruct H0 as [?[??]].
+      subst.
+      revert H1.
+      rewrite /bound/min_val/max_val.
+      intros.
+      rewrite to_unsigned_id; eauto.
+      destruct sz; simpl; try lia.
+    - exfalso. apply H. destruct H0 as [?[??]]. eauto.
+  Qed.
+
+  (* conversion is deterministic *)
+  Lemma conv_int_unique from to v :
+      forall v' v'', conv_int tu from to v v' ->
+                conv_int tu from to v v'' ->
+                v' = v''.
+  Proof using Hmod.
+    rewrite /conv_int.
+    repeat (case_match; try tauto); intuition; try congruence.
+  Qed.
+End conv_int.
+
+(* This (effectively) lifts [conv_int] to arbitrary types.
+
+   TODO: it makes sense for this to mirror the properties of [conv_int], but
+   pointer casts require side-conditions that are only expressible in
+   separation logic.
+ *)
+Definition convert {σ : genv} (tu : translation_unit) (from to : type) (v : val) (v' : val) : Prop :=
+  if is_pointer from && bool_decide (erase_qualifiers from = erase_qualifiers to) then
+    (* TODO: this conservative *)
+    has_type v from /\ has_type v' to /\ v' = v
+  else if is_arithmetic from && is_arithmetic to then
+    conv_int tu from to v v'
+  else False.
