theories/lang/cpp/semantics/cast_operator.v
@@ -1,0 +1,94 @@
+(*
+ * Copyright (c) 2020-23 BedRock Systems, Inc.
+ * This software is distributed under the terms of the BedRock Open-Source License.
+ * See the LICENSE-BedRock file in the repository root for details.
+ *)
+(**
+   Semantics of arithmetic operators on primitives.
+   This does not include the semantics of pointer operations because they
+   require side conditions on the abstract machine state.
+ *)
+
+From bedrock.prelude Require Import base numbers.
+From bedrock.lang.cpp.arith Require Export operator.
+From bedrock.lang.cpp Require Import ast semantics.values semantics.promotion semantics.cast.
+
+#[local] Open Scope Z_scope.
+
+(** ** Binary Operator Static Semantics
+
+    The static (type-level) promotion semantics of binary operators
+  *)
+Notation Tptrdiff_t := Tlonglong (only parsing).
+
+Definition convert_type_op {σ : genv} (tu : translation_unit) (b : BinOp) (ty1 ty2 : type)
+  : option (type * type * type) :=
+  if is_pointer ty1 && is_pointer ty2 then
+    (* pointer-pointer operations *)
+    match b with
+    | Bsub => Some (ty1, ty2, Tptrdiff_t)
+    | _ => None
+    end
+  else if is_pointer ty1 && is_arithmetic ty2 then
+    (* pointer-integer operations *)
+    match b with
+    | Bsub | Badd =>
+      match promote_integral tu ty2 with
+      | Some ty2 => Some (ty1, ty2, ty1)
+      | _ => None
+      end
+    | _ => None
+    end
+  else if is_arithmetic ty1 && is_pointer ty2 then
+    (* integer-pointer operations *)
+    match b with
+    | Bsub | Badd =>
+      match promote_integral tu ty1 with
+      | Some ty1 => Some (ty1, ty2, ty2)
+      | _ => None
+      end
+    | _ => None
+    end
+  else if is_arithmetic ty1 && is_arithmetic ty2 then
+    (* integer-integer operations *)
+    match promote_integral tu ty1 , promote_integral tu ty2 with
+    | Some ity1 , Some ity2 =>
+      match b with
+      | Bshl | Bshr =>
+        (* heterogeneous operators *)
+        Some (ity1, ity2, ity1)
+      | Badd | Bsub | Bmul | Bdiv | Bmod
+      | Band | Bor | Bxor =>
+        (* homogeneous operators *)
+        match promote_arith ity1 ity2 with
+        | Some to => Some (to, to, to)
+        | _ => None
+        end
+      | Beq | Bneq
+      | Blt | Ble | Bgt | Bge =>
+        let same_enum :=
+          match drop_qualifiers ty1 , drop_qualifiers ty2 with
+          | Tenum nm1 , Tenum nm2 => if bool_decide (nm1 = nm2) then true else false
+          | _ , _ => false
+          end
+        in
+        if same_enum then
+          (* Technically, this is only permitted for unscoped enumerations;
+             however, the dynamic semantics lines up with the comparison on
+             scoped enumerations so we do not test.
+           *)
+          Some (drop_qualifiers ty1, drop_qualifiers ty2, Tbool)
+        else
+          (* homogeneous operators *)
+          match promote_arith ity1 ity2 with
+          | Some to => Some (to, to, to)
+          | _ => None
+          end
+      | Bcmp => None
+      | Bdotp
+      | Bdotip
+      | Bunsupported _ => None
+      end
+    | _ , _ => None
+    end
+  else None.
