theories/lang/cpp/semantics/characters.v
@@ -1,0 +1,366 @@
+(*
+ * Copyright (c) 2020-23 BedRock Systems, Inc.
+ * This software is distributed under the terms of the BedRock Open-Source License.
+ * See the LICENSE-BedRock file in the repository root for details.
+ *)
+From elpi Require Import locker.
+
+From bedrock.prelude Require Import base numbers.
+From bedrock.lang.cpp.arith Require Import operator.
+From bedrock.lang.cpp Require Import ast semantics.values.
+
+#[local] Open Scope Z_scope.
+
+(** Architecture independent character values
+
+    To unify the *value* representation of characters, we store characters
+    in an architecture-independent way as [unsigned] integers (using [N]).
+
+    Effectively, this is like storing values of type `char` as if they were
+    `unsigned char` and re-interpreting the bits as `signed char` before
+    performing operations on them. Note that because this is a logical-only
+    conversion, it does not require a boundedness check, i.e. for 8-bit
+    characters, 255 should mean -1 on a signed platform *regardless* of the
+    C++ language version.
+
+    The conversion from this representation to its integral representation
+    is typed *on both sides* meaning that you need both the source and the
+    target type information in order to perfom the conversion.
+
+    The low-level conversion functions are included here to fully document
+    the representation. [conv_int] abstracts these details for use in the
+    rest of the semantics.
+ *)
+
+mlock
+Definition to_char (from_sz : N) (from_sgn : signed) (to_bits : N) (*to_sgn : signed*) (v : Z) : N :=
+  Z.to_N $ v `mod` 2^to_bits.
+
+mlock
+Definition of_char (from_bits : N) (from_sgn : signed) (to_bits : N) (to_sgn : signed) (n : N) : Z :=
+  (* first we need to sign extend using frm_sgn *)
+  let n : Z :=
+    if from_sgn is Signed then
+      if bool_decide (n < 2^(from_bits-1)) then n else to_signed_bits from_bits n
+    else n in
+  if to_sgn is Signed then to_signed_bits to_bits n else to_unsigned_bits to_bits n.
+
+(* suppose that you are in an architecture with unsigned characters
+    and you wrote (128)
+  *)
+Module Type CHAR_TESTS.
+  Goal of_char 8 Signed 32 Signed 1 = 1. Proof. by rewrite of_char.unlock. Qed.
+  Goal of_char 8 Signed 32 Signed 128 = -128. Proof. by rewrite of_char.unlock. Qed.
+  Goal of_char 8 Signed 32 Signed 127 = 127. Proof. by rewrite of_char.unlock. Qed.
+
+  Goal of_char 8 Signed 16 Unsigned 128 = 65408. Proof. by rewrite of_char.unlock. Qed.
+  Goal of_char 32 Signed 8 Signed 256 = 0. Proof. by rewrite of_char.unlock. Qed.
+  Goal of_char 32 Signed 8 Signed 128 = -128. Proof. by rewrite of_char.unlock. Qed.
+  Goal of_char 32 Signed 16 Signed 128 = 128. Proof. by rewrite of_char.unlock. Qed.
+  Goal of_char 16 Signed 8 Unsigned 128 = 128. Proof. by rewrite of_char.unlock. Qed.
+
+  (* Other tests *)
+  Goal of_char 8 Signed 8 Unsigned 128 = 128. Proof. by rewrite of_char.unlock. Qed.
+  Goal of_char 16 Signed 8 Unsigned 128 = 128. Proof. by rewrite of_char.unlock. Qed.
+
+  Goal of_char 8 Signed 8 Signed 128 = -128. Proof. by rewrite of_char.unlock. Qed.
+  Goal of_char 8 Signed 8 Signed 129 = -127. Proof. by rewrite of_char.unlock. Qed.
+
+  Goal of_char 16 Signed 8 Signed 128 = -128. Proof. by rewrite of_char.unlock. Qed.
+  Goal of_char 16 Signed 8 Signed 129 = -127. Proof. by rewrite of_char.unlock. Qed.
+
+  Goal of_char 8 Unsigned 8 Signed 129 = -127. Proof. by rewrite of_char.unlock. Qed.
+  Goal of_char 16 Unsigned 8 Signed 129 = -127. Proof. by rewrite of_char.unlock. Qed.
+
+  Goal of_char 8 Unsigned 8 Signed 128 = -128. Proof. by rewrite of_char.unlock. Qed.
+  Goal of_char 8 Unsigned 16 Signed 128 = 128. Proof. by rewrite of_char.unlock. Qed.
+
+  Goal of_char 4 Signed 8 Unsigned 8 = 248. Proof. by rewrite of_char.unlock. Qed.
+  Goal to_char 8 Unsigned 4 248 = 8%N. Proof. by rewrite to_char.unlock. Qed.
+
+  Goal of_char 8 Signed 16 Signed 129 = -127%N. Proof. by rewrite of_char.unlock; compute. Qed.
+  Goal to_char 16 Signed 8 (-127)%Z = 129%N. Proof. by rewrite to_char.unlock; compute. Qed.
+
+  Goal of_char 8 Signed 4 Signed 17 = 1%N. Proof. by rewrite of_char.unlock; compute. Qed.
+End CHAR_TESTS.
+
+
+Lemma of_char_spec_low (from_bits : N) (from_sgn : signed)
+  (to_bits : N) (to_sgn : signed) (v : N) :
+  (from_bits ≤ to_bits)%Z
+  -> (0 <= v < 2 ^ (from_bits - 1))%Z
+  -> of_char from_bits from_sgn to_bits to_sgn v = v.
+Proof.
+  move=>Ho [Hlb Hub].
+
+  have Hsz : (v < 2 ^ (to_bits - 1))%Z.
+  { apply: Z.lt_le_trans; first done.
+    by apply: Z.pow_le_mono; lia. }
+
+  have Hop : (2 ^ (from_bits - 1) ≤ 2 ^ to_bits)%Z
+    by apply: Z.pow_le_mono; lia.
+
+  rewrite of_char.unlock.
+  case Hs: from_sgn.
+  - case: bool_decide_reflect; last by done.
+    case: to_sgn=>?; first by apply: to_signed_bits_id.
+    by rewrite /trim Z.mod_small; lia.
+  - case: to_sgn; first by apply: to_signed_bits_id; lia.
+    by rewrite /= /trim Z.mod_small //; lia.
+Qed.
+
+Definition of_char_specf from_bits from_sgn to_bits to_sgn (v : Z) : Z :=
+  match to_sgn with
+  | Signed => match from_sgn with
+             | Signed => (v - 2 ^ from_bits)%Z
+             | Unsigned =>
+                 if bool_decide (from_bits = to_bits) then
+                   (v - 2 ^ from_bits)%Z else v
+             end
+  | Unsigned => match from_sgn with
+             | Signed => (v - 2 ^ from_bits + 2 ^ to_bits)%Z
+             | Unsigned => v
+             end
+  end.
+
+Lemma of_char_spec_high (from_bits : N) (from_sgn : signed) (to_bits : N) (to_sgn : signed) (v : N) :
+  (0 < from_bits)%Z
+  -> (from_bits ≤ to_bits)%Z
+  -> (2 ^ (from_bits - 1) <= v < 2 ^ from_bits)%Z
+  -> of_char from_bits from_sgn to_bits to_sgn v =
+      of_char_specf from_bits from_sgn to_bits to_sgn v.
+Proof.
+  move=>Hbits Ho; rewrite of_char.unlock /of_char_specf.
+  case Hfs: from_sgn.
+  - case: bool_decide_reflect; first by lia.
+    move=>? [??]; case Htf: to_sgn.
+    + rewrite [to_signed_bits _ v]to_signed_bits_spec_high;
+        try by [ lia | case: (from)].
+      rewrite to_signed_bits_spec_low //; split.
+      * rewrite -Z.le_add_le_sub_l.
+        apply: Z.le_trans; last done.
+
+        rewrite Z.le_add_le_sub_r Z.sub_opp_r -Z.le_sub_le_add_l.
+        rewrite Z_pow2_half; last lia.
+        rewrite Z.add_simpl_r; apply: Z.pow_le_mono; lia.
+      * rewrite Z.lt_sub_lt_add_l.
+        apply: Z.lt_le_trans; first done.
+        by lia.
+
+    + rewrite to_signed_bits_spec_high; try by [| lia].
+      rewrite /trim Z_mod_big //; split; last lia.
+      rewrite -Z.le_add_le_sub_l; apply: Z.le_trans; last done.
+
+
+      rewrite Z_pow2_half; last lia.
+      rewrite -Z.add_assoc Z.le_add_le_sub_l.
+      apply: Zplus_le_compat_l; rewrite -Z.opp_le_mono;
+        apply: Z.pow_le_mono; lia.
+
+  - move: Ho=>/Zle_lt_or_eq[Hlt[??]/=|].
+    + case: to_sgn.
+      * rewrite to_signed_bits_spec_low.
+
+        case: bool_decide_reflect Hlt; by [lia |].
+
+        split; first by apply: Z.le_trans; by [| lia].
+        apply: Z.lt_le_trans; first by done.
+        by apply: Z.pow_le_mono; lia.
+
+      * rewrite /trim Z.mod_small //.
+        split; first by lia.
+        apply: Z.lt_le_trans; first done.
+        apply: Z.pow_le_mono; lia.
+
+    + move=>Heq; rewrite Heq. move=>[??].
+      case: to_sgn; last
+        by rewrite /trim Z.mod_small //; lia.
+      case: bool_decide_reflect Heq Hbits=>???; last done.
+      rewrite to_signed_bits_spec_high; lia.
+Qed.
+
+Lemma to_char_spec_low (from_bits : N) (from_sgn : signed) (to_bits : N) (v : Z) :
+  (0 <= v < 2 ^ to_bits)%Z
+  -> to_char from_bits from_sgn to_bits v = Z.to_N v.
+Proof.
+  rewrite to_char.unlock.
+  intros. by rewrite Z.mod_small.
+Qed.
+
+Lemma to_char_spec_high (from_bits : N) (from_sgn : signed) (to_bits : N) (to_sgn : signed) (v : Z) :
+  (from_bits ≤ to_bits)%Z
+  -> (2 ^ from_bits | 2 ^ to_bits)%Z
+  -> (2 ^ (from_bits - 1) <= v < 2 ^ from_bits)%Z
+  -> to_char to_bits to_sgn from_bits
+      (of_char_specf from_bits from_sgn to_bits to_sgn v) = (Z.to_N v).
+Proof.
+  move=>Ho Hd [Hlb Hub].
+  have Hpow: (2 ^ from_bits <= 2 ^ to_bits)%Z
+    by apply: Z.pow_le_mono.
+  have Hlt: (v < 2 ^ to_bits)%Z
+    by apply: Z.lt_le_trans.
+
+  rewrite to_char.unlock // /trim /of_char_specf.
+  case Hts: to_sgn.
+  + case: from_sgn; first
+      by rewrite Z_mod_big; lia.
+    case: bool_decide_reflect; first
+      by move=>->; rewrite Z_mod_big; lia.
+    by rewrite Z.mod_small; lia.
+  +
+    case Hfs: from_sgn; last
+      by rewrite Z.mod_small; lia.
+
+    rewrite Zplus_mod.
+    move: Hd; rewrite -Z.mod_divide; last lia.
+    move=>->; rewrite Z.add_0_r.
+    rewrite Z.mod_mod; last lia.
+    by rewrite Z_mod_big; lia.
+Qed.
+
+Lemma of_char_to_char (from_bits : N) (from_sgn : signed) (to_bits : N)
+  (to_sgn : signed) (v : N) :
+  (0 < from_bits)%Z
+  -> (from_bits ≤ to_bits)%Z
+  -> (2 ^ from_bits | 2 ^ to_bits)%Z
+  -> (0 <= v < 2 ^ from_bits)%Z
+  -> to_char to_bits to_sgn from_bits
+          (of_char from_bits from_sgn to_bits to_sgn v) = v.
+Proof.
+  move=>H0 Ho Hd [Hlb Hub].
+  case: (Z.lt_ge_cases v (2 ^ (from_bits - 1))%Z)=>[?|?].
+  - by rewrite of_char_spec_low // to_char_spec_low; lia.
+  - by rewrite of_char_spec_high // to_char_spec_high // N2Z.id.
+Qed.
+
+Lemma of_char_trim (from_bits to_bits : N) (v : Z) :
+  (to_bits <> 0%N)
+  -> (to_bits <= from_bits)%Z
+  -> (2 ^ (to_bits - 1) ≤ v < 2 ^ to_bits)
+  -> (2 ^ from_bits | 2 ^ to_bits)
+  -> of_char to_bits Signed from_bits Unsigned (Z.to_N (trim to_bits v)) = v.
+Proof.
+  move=>??[??]?.
+  have H2: (2 ^ to_bits <= 2 ^ from_bits)%Z
+    by apply: Z.pow_le_mono.
+
+  rewrite of_char.unlock /=.
+
+  case: bool_decide_reflect; first
+    by rewrite /trim Z.mod_small; lia.
+  move=>/Znot_lt_ge/Z.ge_le ?.
+
+  rewrite /to_signed_bits.
+  case: bool_decide_reflect=>[|?]; first lia.
+  case: bool_decide_reflect=>[?|]; last first.
+  - move=>/Znot_ge_lt.
+    rewrite Z.mod_small;try lia.
+    rewrite /trim Z.mod_small;try lia.
+  -
+    rewrite /trim Z2N.id (Z.mod_small v); try lia.
+    rewrite (Z.mod_small v); last lia.
+    apply: Znumtheory.Zdivide_mod_minus; try lia.
+
+    rewrite -Z.sub_add_distr Z.add_comm Z.sub_add_distr.
+    rewrite Z.sub_diag Z.sub_0_l.
+    by apply: Znumtheory.Zdivide_opp_r.
+Qed.
+
+(* architecture-dependent domain where [to_char] is left inverse of [of_char] *)
+#[program]
+Definition to_char_domP (from_bits : N) (from_sgn : signed) to_bits to_sgn (v : Z) : Prop :=
+  match to_sgn with
+  | Signed =>  match from_sgn with
+              | Signed => (- 2 ^ (to_bits - 1) <= v < 2 ^ (to_bits - 1))%Z
+              | Unsigned => (0 <= v < 2 ^ to_bits)%Z /\ (2 ^ from_bits | 2 ^ to_bits)
+              end
+  | Unsigned => match from_sgn with
+               | Signed =>
+                   if bool_decide (to_bits = from_bits) then
+                     (- 2 ^ (to_bits - 1) <= v < 2 ^ (to_bits - 1))%Z
+                   else
+                     (0 <= v < 2 ^ to_bits)%Z
+               | Unsigned => (0 <= v < 2 ^ to_bits)%Z
+               end
+  end.
+
+Lemma to_char_of_char (from_bits : N) (from_sgn : signed) (to_bits : N)
+  (to_sgn : signed) (v : Z) :
+  (0 < to_bits)%Z
+  -> (to_bits ≤ from_bits)%Z
+  -> to_char_domP from_bits from_sgn to_bits to_sgn v
+  -> of_char to_bits to_sgn from_bits from_sgn
+      (to_char from_bits from_sgn to_bits v) = v.
+Proof.
+  move=>H0 Ho.
+
+  have H1: (2 ^ (to_bits - 1) < 2 ^ to_bits)%Z
+    by apply: Z.pow_lt_mono_r; lia.
+  have H2: (2 ^ to_bits <= 2 ^ from_bits)%Z
+    by apply: Z.pow_le_mono.
+
+  rewrite to_char.unlock //.
+
+  case: to_sgn.
+  - case: from_sgn=>[/=?|[??]].
+
+    + case: (Z.lt_ge_cases v 0)%Z=>[?|?].
+      rewrite /trim Z_mod_big; last lia.
+      rewrite of_char_spec_high /=; try lia.
+      rewrite (Z_pow2_half to_bits); lia.
+      rewrite /trim Z.mod_small; last lia.
+      rewrite of_char_spec_low; lia.
+    +
+      case: (Z.lt_ge_cases v ((2 ^ (to_bits - 1)))%Z)=>[?|?].
+      rewrite /trim Z.mod_small; last lia.
+      rewrite of_char_spec_low; try lia.
+      by rewrite of_char_trim; try lia.
+
+  - case: from_sgn=>[/=|[??]].
+    + case: bool_decide_reflect=>[/N2Z.inj Heq [??]|Heq [??]].
+
+      * case: (Z.lt_ge_cases v 0)%Z=>[?|?].
+        rewrite /trim Z_mod_big /=; last lia.
+        rewrite of_char_spec_high /=; try lia.
+        case: bool_decide_reflect Heq; lia.
+        rewrite (Z_pow2_half to_bits); lia.
+        rewrite /trim Z.mod_small /=; last lia.
+        rewrite of_char_spec_low; lia.
+      * rewrite /trim Z.mod_small; last lia.
+        case: (Z.lt_ge_cases v ((2 ^ (to_bits - 1)))%Z)=>[?|?].
+        rewrite of_char_spec_low; lia.
+        rewrite of_char_spec_high /=; try lia.
+        case: bool_decide_reflect Heq; lia.
+    + rewrite /trim Z.mod_small; last lia.
+      case: (Z.lt_ge_cases v ((2 ^ (to_bits - 1)))%Z)=>[?|?].
+      rewrite of_char_spec_low; lia.
+      rewrite of_char_spec_high /=; lia.
+Qed.
+
+Lemma to_char_bounded sz sgn bits z :
+  (to_char sz sgn bits z < 2^bits)%N.
+Proof.
+  rewrite to_char.unlock.
+  generalize (Z_mod_lt z (2^bits)). lia.
+Qed.
+
+Lemma of_char_bounded (from_sz : N) from_sgn (to_sz : N) to_sgn n :
+  0 < to_sz -> 0< from_sz ->
+  let min_val : Z := if to_sgn is Signed then -2^(to_sz-1) else 0 in
+  let max_val : Z := if to_sgn is Signed then 2^(to_sz-1) else 2^to_sz in
+  min_val <= of_char from_sz from_sgn to_sz to_sgn n < max_val.
+Proof.
+  rewrite of_char.unlock /to_signed_bits; intros.
+  assert (2^to_sz = 2 * 2^(to_sz - 1)).
+  { have->: Z.of_N to_sz = Z.succ (to_sz - 1) by lia.
+    rewrite Z.pow_succ_r; try lia. f_equal. f_equal. lia. }
+  #[local] Ltac saturate :=
+    repeat match goal with
+      | |- context [ Z.modulo ?X ?Y ] =>
+          lazymatch goal with
+          | H : (0 <= X `mod` Y < Y)%Z |- _ => fail 1
+          | |- _ => generalize (Z.mod_pos_bound X Y ltac:(lia)); intro
+          end
+      end.
+  repeat first [ case_bool_decide | case_match ]; rewrite /trim/=; split; try rewrite Zmod_0_l ; saturate; try lia.
+Qed.
