theories/lang/cpp/semantics/promotion.v
@@ -1,0 +1,244 @@
+(*
+ * Copyright (c) 2020-22 BedRock Systems, Inc.
+ * This software is distributed under the terms of the BedRock Open-Source License.
+ * See the LICENSE-BedRock file in the repository root for details.
+ *)
+(** * Type-level semantics of type promotions
+
+    This captures the rules that C++ uses to promote values to integral types for
+    the purposes of performing computation.
+
+    This file contains *only* static-semantics, i.e. determining what casts should
+    be performed. The dynamic semantics of casts is defined in [semantics/cast.v]
+ *)
+
+From bedrock.prelude Require Import base numbers.
+From bedrock.lang.cpp.arith Require Export operator.
+From bedrock.lang.cpp Require Import ast semantics.values.
+
+#[local] Open Scope Z_scope.
+
+(** [underlying_type tu nm] is the type that underlies [Tenum nm].
+ *)
+Definition underlying_type (tu : translation_unit) (nm : globname) : option type :=
+  match tu.(globals) !! nm with
+  | Some (Genum ty _) => Some $ drop_qualifiers ty
+  | _ => None
+  end.
+
+(** [representation_type tu ty] is the type that underlies [ty] if [ty] is an [enum],
+    otherwise, it is the orginal type.
+
+    Note that if the [enum] is not defined in the translation unit, then the result
+    it the original [enum].
+ *)
+Definition representation_type (tu : translation_unit) (ty : type) : type :=
+  match drop_qualifiers ty with
+  | Tenum nm as ty => default ty $ underlying_type tu nm
+  | ty => ty
+  end.
+
+Succeed Example underlying_int : forall tu, representation_type tu Tint = Tint :=
+  ltac:(compute; auto).
+Succeed Example underlying_int : forall tu, representation_type tu (Qconst Tint) = Tint :=
+  ltac:(compute; auto).
+
+(*
+(** [underlying_unqual_type tu ty] is the unqualified type that underlies [ty].
+
+    This is the strip qualifiers function if [ty] is not an `enum`.
+
+ *)
+Definition underlying_unqual_type (tu : translation_unit) (ty : type) : type :=
+  let '(cv, ty') := decompose_type ty in
+  match ty' with
+  | Tenum nm as ty =>
+      match tu.(globals) !! nm with
+      | Some (Genum ty _) => ty
+      | _ => ty'
+      end
+  | _ => ty'
+  end.
+
+Succeed Example underlying_int : forall tu, underlying_unqual_type tu (Qconst Tint) = Tint :=
+  ltac:(compute; auto).
+*)
+
+Section representable.
+  Context {σ : genv}.
+  (* [fully_representable a b] is [true] if all (well-typed) values of [a] values of [b] *)
+  Definition fully_representable (a b : type) : bool :=
+    let to_equiv ty :=
+      match ty with
+      | Tnum a b => Some $ integral_type.mk a b
+      | Tchar_ ct => Some $ equivalent_int_type _ ct
+      | _ => None
+      end
+    in
+    let min ty := (fun '(integral_type.mk sz sgn) => min_val sz sgn) <$> to_equiv ty in
+    let max ty := (fun '(integral_type.mk sz sgn) => max_val sz sgn) <$> to_equiv ty in
+    match min a , min b , max a , max b with
+    | Some an , Some bn , Some ax , Some bx =>
+        bool_decide (bn <= an /\ ax <= bx)%Z
+    | _ , _ , _ , _ => false
+    end.
+
+  (* [first_representable ty ls] gets the first type in [ls] that is able to
+     fully represent [ty]
+   *)
+  Fixpoint first_representable (ty : type) (ls : list type) : option type :=
+    match ls with
+    | nil => None
+    | l :: ls => if fully_representable ty l then Some l else first_representable ty ls
+    end.
+End representable.
+
+(** ** Integral Promotion
+    This is used to promote a type to a type that supports arithmetic operators.
+    For example, it converts types smaller than `int` to `int` (of some signedness).
+    Because it converts `enum` types to integral types, it takes a [translation_unit].
+
+    The operation is partial for non-integral types, e.g. struct types.
+
+    Note that integral promotion does *not* change the value in the C++ semantics;
+    however, it does change from [Vchar] to an equivalent [Vint] in BRiCk's
+    architecture-independent semantics.
+
+    > A prvalue of an integer type other than `bool`, `char8_t`, `char16_t`,
+    > `char32_t`, or `wchar_t` whose integer conversion rank ([conv.rank])
+    > is less than the rank of `int` can be converted to a prvalue of type `int`
+    > if int can represent all the values of the source type; otherwise, the
+    > source prvalue can be converted to a prvalue of type `unsigned int`.
+
+    <https://eel.is/c++draft/conv.prom>
+
+ *)
+Definition promote_integral {σ : genv} (tu : translation_unit) (ty : type) : option type :=
+  match representation_type tu ty with
+    (* signed char or short can be converted to int *)
+  | Tschar
+  | Tshort => Some Tint
+    (* unsigned char or unsigned short can be converted to int if it can hold its entire
+        value range, and unsigned int otherwise *)
+  | Tuchar as ty
+  | Tushort as ty => Some $ if fully_representable ty Tint then Tint else Tuint
+  | Tnum _ _ as ty => Some ty
+  | Tchar =>
+      Some $ let rty := if σ.(char_signed) is Signed then Tschar else Tuchar in
+             if fully_representable rty Tint then Tint else Tuint
+  | Twchar
+  | Tchar_ char_type.C8
+  | Tchar_ char_type.C16
+  | Tchar_ char_type.C32 =>
+    (* wchar_t, char8_t (since C++20), char16_t, and char32_t
+       (since C++11) can be converted to the first type from the
+       following list able to hold their entire value range: int,
+       unsigned int, long, unsigned long, long long,
+       unsigned long long (since C++11) *)
+
+      first_representable ty [Tint;Tuint;Tlong;Tulong;Tlonglong;Tulonglong]
+  | Tenum nm => None
+      (* unreachable because of [underlying_type] and because the
+          underlying type of an `enum` must be a fundamental type. *)
+      (* an unscoped enumeration type whose underlying type
+        is not fixed can be converted to the first type from the following
+        list able to hold their entire value range: int, unsigned int, long,
+        unsigned long, long long, or unsigned long long, extended integer
+        types with higher conversion rank (in rank order, signed given
+        preference over unsigned) (since C++11). If the value range is
+        greater, no integral promotions apply;
+
+        an unscoped enumeration type whose underlying type is
+        fixed can be converted to its underlying type, and, if the
+        underlying type is also subject to integral promotion, to the
+        promoted underlying type. Conversion to the unpromoted underlying
+        type is better for the purposes of overload resolution)
+
+        NOTE: this only applies to `unscoped` enumerations; however, the
+        program will never contain these sorts of implicit conversions for
+        scoped enumerations, so we do not need to check this fact.
+          *)
+  | Tbool => Some Tint
+  | Tptr _
+  | Tref _
+  | Trv_ref _
+  | Tvoid
+  | Tarray _ _
+  | Tnamed _
+  | Tfunction _ _
+  | Tmember_pointer _ _
+  | Tfloat _
+  | Tnullptr
+  | Tarch _ _ => None
+  | Tqualified _ _ => None (* unreachable *)
+  end.
+
+Goal forall {σ : genv} tu, promote_integral tu Tchar = Some Tint.
+Proof.
+  intros. rewrite /promote_integral/=.
+  destruct (char_signed σ); done.
+Succeed Qed. Abort.
+Goal forall {σ : genv} tu, promote_integral tu Twchar = Some (integral_type.to_type $ equivalent_int_type _ char_type.Cwchar).
+Proof.
+  intros. rewrite /promote_integral/equivalent_int_type/=.
+  rewrite /fully_representable/=.
+  destruct (wchar_signed σ); done.
+Succeed Qed. Abort.
+
+(* Test cases *)
+Succeed Example promote_short : forall {σ : genv} tu,
+    promote_integral tu Tshort = Some Tint :=
+  ltac:(compute; reflexivity).
+Succeed Example promote_uchar : forall {σ : genv} tu,
+    promote_integral tu Tuchar = Some Tint :=
+  ltac:(compute; reflexivity).
+Succeed Example promote_schar : forall {σ : genv} tu,
+    promote_integral tu Tschar = Some Tint :=
+  ltac:(compute; reflexivity).
+
+(** ** Arithmetic Promotion
+  This computes a "join" on the types of the two arguments to an arithmetic
+  operator.
+
+  https://eel.is/c++draft/expr.arith.conv#1.3
+
+  (1.3.1) If both operands have the same type, no further conversion is needed.
+  (1.3.2) Otherwise, if both operands have signed integer types or both have
+          unsigned integer types, the operand with the type of lesser integer
+          conversion rank is converted to the type of the operand with greater
+          rank.
+  (1.3.3) Otherwise, if the operand that has unsigned integer type has rank
+          greater than or equal to the rank of the type of the other operand,
+          the operand with signed integer type is converted to the type of the
+          operand with unsigned integer type.
+  (1.3.4) Otherwise, if the type of the operand with signed integer type can
+          represent all of the values of the type of the operand with unsigned
+          integer type, the operand with unsigned integer type is converted to
+          the type of the operand with signed integer type.
+  (1.3.5) Otherwise, both operands are converted to the unsigned integer type
+          corresponding to the type of the operand with signed integer type.
+  *)
+Definition promote_arith (ty1 ty2 : type) : option type :=
+  match ty1 , ty2 with
+  | Tnum sz1 sgn1 , Tnum sz2 sgn2 =>
+      if bool_decide (sgn1 = sgn2) then
+        Some $ Tnum (int_type.t_max sz1 sz2) sgn1
+      else
+        let (ssz, usz) := match sgn1 with
+                          | Signed => (sz1, sz2)
+                          | Unsigned => (sz2, sz1)
+                          end
+        in
+        if bool_decide (int_type.t_le ssz usz) then
+          Some $ Tnum usz Unsigned
+        else if bool_decide (int_type.t_le usz ssz) then
+          Some $ Tnum ssz Signed
+        else
+          Some $ Tnum ssz Unsigned
+  | _ , _ => None
+  end.
+
+(* Test cases *)
+Succeed Example promote_int_long : promote_arith Tint Tlong = Some Tlong := eq_refl.
+Succeed Example promote_int_ulong : promote_arith Tint Tulong = Some Tulong := eq_refl.
+Succeed Example promote_uint_long : promote_arith Tuint Tlong = Some Tlong := eq_refl.
